thinking about well foundedness

theorems/main.v
@@ -1,11 +1,92 @@
-Require Import List String.
+Add LoadPath "/home/blaine/personal/cpdtlib" as Cpdt.
+Set Implicit Arguments. Set Asymmetric Patterns.
+Require Import List String Cpdt.CpdtTactics.
+From stdpp Require Import base fin vector options.
 Import ListNotations.
 
-From stdpp Require Import base fin vector options.
+Ltac solve_crush := try solve [crush].
+Ltac solve_assumption := try solve [assumption].
+Ltac subst_injection H := injection H; intros; subst; clear H.
+
+Theorem valid_index_not_None {T}: forall (l: list T) index,
+	index < (length l) -> (lookup index l) <> None.
+Proof.
+	intros ????%lookup_ge_None; lia.
+Qed.
+Theorem valid_index_Some {T}: forall (l: list T) index,
+	index < (length l) -> exists t, (lookup index l) = Some t.
+Proof.
+	intros ???%(lookup_lt_is_Some_2 l index);
+	unfold is_Some in *; assumption.
+Qed.
+
+Definition closer_to target: nat -> nat -> Prop :=
+	fun next cur => (target - next) < (target - cur).
+(*Hint Unfold closer_to: core.*)
+
+Theorem closer_to_well_founded target: well_founded (closer_to target).
+Proof.
+	apply (well_founded_lt_compat nat (fun a => target - a)); intros; assumption.
+Defined.
+
+Theorem closer_to_reverse: forall target cur next,
+	(target - next) < (target - cur) -> cur < next.
+Proof. lia. Qed.
+
+Theorem closer_to_bounded_reverse: forall target cur next,
+	cur < next -> cur < target -> (target - next) < (target - cur).
+Proof. lia. Qed.
+
+Definition closer_to_end {T} (arr: list T) := closer_to (length arr).
+
+Theorem closer_to_end_well_founded {T} (arr: list T): well_founded (closer_to_end arr).
+Proof. apply closer_to_well_founded. Qed.
+
+
+Section well_founded_compatibility.
+	Variable A B: Type.
+	Variable RA: A -> A -> Prop.
+	Variable RB: B -> B -> Prop.
+
+	Variable RB_well_founded: well_founded RB.
+	Variable f: A -> B.
+	Hypothesis H_compat: forall a1 a2: A, RA a1 a2 <-> RB (f a1) (f a2).
+
+	Theorem well_founded_compat: well_founded RA.
+	Proof.
+constructor.
+
+unfold well_founded in *.
+constructor.
+intros.
+rename y into a1; rename a into a2.
+
+specialize (H_compat a1 a2).
+remember (f a1) as b1; remember (f a2) as b2.
+destruct H_compat as [H_compat_A H_compat_B].
+specialize (H_compat_A H) as ?.
+
+
+specialize (RB_well_founded b1) as Hb1.
+specialize (RB_well_founded b2) as Hb2.
+inversion Hb1.
+
+
+specialize (Acc_inv RB_well_founded).
+
+	Qed.
+
+Check RB_well_founded.
+
+EndSection well_founded_compatibility.
+
+(*
+forall (?A ?B: Type) (?RA: ?A -> ?A -> Prop) (?RW: ?B -> ?B -> Prop) -> _
+*)
+
 
 Example t1: ([# 4; 2] !!! 0%fin) = 4.
 Proof. reflexivity. Qed.
-
 
 Section Sized.
 	Variable size: nat.
@@ -28,52 +109,210 @@ Section Sized.
 
 	(*Definition label := option string.*)
 	Inductive Instruction :=
+		| InstExit
 		| InstMov (src: Operand) (dest: register)
 		| InstAdd (val: Operand) (dest: register)
-		(*| InstBranchEq (a: Operand) (b: Operand) (to: label)*)
-		(*| InstBranchNeq (a: Operand) (b: Operand) (to: label)*)
-		| InstExit
-	.
 
-	(*Record State := state { counter: nat; bank: RegisterBank }.*)
+		(*| InstJump (to: string)*)
+		(*| InstBranchEq (a: Operand) (b: Operand) (to: string)*)
+		(*| InstBranchNeq (a: Operand) (b: Operand) (to: string)*)
+
+		(*| InstStore (src: Operand) (dest: Operand)*)
+		(*| InstLoad (src: Operand) (dest: register)*)
+	.
+	Hint Constructors Instruction: core.
+
+	Inductive branching: Instruction -> Prop :=
+		(*| branch_BranchEq: forall a b to, branching (InstBranchEq a b to)*)
+		(*| branch_BranchNeq: forall a b to, branching (InstBranchNeq a b to)*)
+		(*| branch_Jump: forall to, branching (InstJump to)*)
+	.
+	Hint Constructors branching: core.
+
+	Inductive terminating: Instruction -> Prop :=
+		| terminating_Exit: terminating InstExit
+	.
+	Hint Constructors terminating: core.
+
+	(*Notation "'appear' instr program cur" :=
+		((lookup cur program) = Some instr) (at level 70).*)
+
+	Record MachineState := state {
+		counter: nat;
+		registers: RegisterBank
+	}.
 
 	Inductive step
-		{program: list Instruction} {counter} {bank}
+		{program: list Instruction} {cur} {bank}
 	: nat -> RegisterBank -> Prop :=
 		| step_Mov: forall src dest,
-			(lookup counter program) = Some (InstMov src dest)
+			(lookup cur program) = Some (InstMov src dest)
 			-> step
-				(S counter)
+				(S cur)
 				(vinsert dest (eval_operand bank src) bank)
+
 		| step_Add: forall val dest,
-			(lookup counter program) = Some (InstAdd val dest)
+			(lookup cur program) = Some (InstAdd val dest)
 			-> step
-				(S counter)
+				(S cur)
 				(vinsert dest ((eval_operand bank val) + (bank !!! dest)) bank)
+
+		(*| step_Jump: forall to,
+			(lookup cur program) = Some (InstJump to)
+			-> exists next, find_label program to = Some next
+			-> step next bank*)
+
+		(*| step_BranchEq_Eq: forall a b to,
+			(lookup cur program) = Some (InstBranchEq a b to)
+			-> a = b
+			-> exists next, find_label program to = Some next
+			-> step next bank
+		| step_BranchEq_Neq: forall a b to,
+			(lookup cur program) = Some (InstBranchEq a b to)
+			-> a <> b
+			-> step (S cur) bank*)
+
+		(*| step_BranchNeq_Neq: forall a b to,
+			(lookup cur program) = Some (InstBranchNeq Ne b to)
+			-> a <> b
+			-> exists next, find_label program to = Some next
+			-> step next bank
+		| step_BranchNeq_Eq: forall a b to,
+			(lookup cur program) = Some (InstBranchNeq Ne b to)
+			-> a = b
+			-> step (S cur) bank*)
 	.
 	Hint Constructors step: core.
 
-	Theorem step_pointing_not_stuck: forall (program: list Instruction) counter bank i,
-		(lookup counter program) = Some i
-		-> (i = InstExit) \/ exists counter' bank', @step program counter bank counter' bank'.
+	Theorem terminating_stuck instr:
+		terminating instr
+		-> (
+			forall program cur next b1 b2, (lookup cur program) = Some instr
+			-> ~(@step program cur b1 next b2)
+		).
 	Proof.
-		intros ??? [] ?; try solve [auto]; right; eauto.
+		intros Hterminating ?????? Hstep;
+		inversion Hterminating; inversion Hstep; crush.
 	Qed.
+
+	(*
+	Inductive Acc (R: A -> A -> Prop) x: Prop :=
+		Acc_intro: (forall y, R y x -> Acc R y) -> Acc R x
+	*)
+
+	Definition program_counter_well_founded program :=
+		(*well_founded (fun next cur => exists b1 b2, @step program cur b1 next b2).*)
+		forall b1 b2, well_founded (fun next cur => @step program cur b1 next b2).
+
+	Inductive terminated: list Instruction -> Prop :=
+		| terminated_End: forall instr,
+			terminating instr
+			-> terminated [instr]
+
+		| terminated_Cons: forall instr rest,
+			~(branching instr)
+			-> ~(terminating instr)
+			-> terminated rest
+			-> terminated (instr :: rest)
+	.
+	Hint Constructors terminated: core.
+
+	Theorem terminated_step_increments program:
+		terminated program
+		-> forall cur next b1 b2, @step program cur b1 next b2
+		-> next = S cur.
+	Proof.
+		intros Hterminated ???? Hstep;
+		inversion Hterminated; inversion Hstep; crush.
+	Qed.
+
+	(*
+	*)
+
+
+	Theorem terminated_always_terminates: forall program,
+		terminated program
+		-> program_counter_well_founded program.
+	Proof.
+unfold program_counter_well_founded.
+intros.
+induction H.
+-
+specialize (terminating_stuck H).
+intros.
+constructor.
+
++
+crush.
+constructor.
+intros.
+unfold not in H.
+specialize (H0 H).
+apply H0 in H.
+
+apply H0 in H.
+
+
+intros.
+
+
+-
+
+constructor.
+
+(*
+either terminated shows that we only have one terminating instruction left, in which case no step can be produced and so this is the root
+or
+*)
+
+apply (well_founded_lt_compat nat (fun a => target - a)).
+
+intros ?. induction 1.
+
+-
+
+
+
+	Qed.
+
+
+	Theorem existent_not_stuck: forall program cur bank instr,
+		(lookup cur program) = Some instr
+		->
+			terminating instr
+			\/ exists cur' bank', @step program cur bank cur' bank'.
+	Proof. intros ??? [] ?; eauto. Qed.
+
+	Theorem terminated_wf: forall program,
+		terminated program
+		->
+		-> well_founded (remaining)
+
+	Theorem terminated_not_stuck: forall program,
+		terminated program
+		->
+
+		(lookup cur program) = Some instr
+		->
+			terminating instr
+			\/ exists next bank', @step program cur bank next bank'.
+	Proof. intros ??? [] ?; eauto. Qed.
+
 
 	Fixpoint execute_program_unsafe
 		(fuel: nat) (program: list Instruction)
-		(counter: nat) (bank: RegisterBank)
+		(cur: nat) (bank: RegisterBank)
 	: option RegisterBank :=
-		match (lookup counter program) with
+		match (lookup cur program) with
 		| None => None
 		| Some i => match fuel, i with
 			| _, InstExit => Some bank
 			| 0, _ => None
 			| S f, InstMov src dest => execute_program_unsafe
-				f program (S counter)
+				f program (S cur)
 				(vinsert dest (eval_operand bank src) bank)
 			| S f, InstAdd val dest => execute_program_unsafe
-				f program (S counter)
+				f program (S cur)
 				(vinsert dest ((eval_operand bank val) + (bank !!! dest)) bank)
 			end
 		end
@@ -147,10 +386,10 @@ Notation expr := Instruction (only parsing).
 Notation of_val := InstExit (only parsing).
 
 Definition to_val (e: expr): option val :=
-  match e with
-  | InstExit _ v => Some v
-  | _ => None
-  end.
+	match e with
+	| InstExit _ v => Some v
+	| _ => None
+	end.
 
 (*
 	So the first program I'm interested in verifying is this one.
